src/lib/kuiper/Kuiper.Math.Fmin.fst
@@ -4,10 +4,32 @@ open Kuiper.IntAliases
 open Kuiper.Scalars.Base
 open Kuiper.Floating.Base
 open Kuiper.Float32
-open Kuiper.Functions
+open Kuiper.Seq.Common
+module Seq = FStar.Seq
 
-let fmin_assoc : squash (is_associative (fmin #f32)) = admit()
-let fmin_comm : squash (is_commutative (fmin #f32)) = admit()
-let fmin_pos_inf_neutral
-  : squash (is_neutral_for pos_inf (fmin #f32))
-  = admit()
+let rec seq_fold_left_append
+  (#a #b : Type) (f : b -> a -> b) (acc : b)
+  (l0 l1 : Seq.seq a)
+  : Lemma (ensures seq_fold_left f acc (Seq.append l0 l1) ==
+                   seq_fold_left f (seq_fold_left f acc l0) l1)
+          (decreases Seq.length l0)
+  = match view_seq l0 with
+    | SNil -> assert (Seq.equal (Seq.append l0 l1) l1)
+    | SCons hd tl ->
+      let SCons hd' tl' = view_seq (Seq.append l0 l1) in
+      assert (hd == hd');
+      assert (Seq.equal tl' (Seq.append tl l1));
+      seq_fold_left_append f (f acc hd) tl l1
+
+let seq_fold_left_one
+  (#a #b : Type) (f : b -> a -> b) (acc : b) (x : a)
+  : Lemma (seq_fold_left f acc (Seq.create 1 x) == f acc x)
+  = let s : Seq.seq a = Seq.create 1 x in
+    assert (Seq.length s == 1);
+    assert (Seq.head s == x);
+    Seq.lemma_eq_intro (Seq.tail s) Seq.empty
+
+let seq_fmin_snoc (s : Seq.seq f32) (x : f32)
+  : Lemma (seq_fmin (Seq.snoc s x) == fmin (seq_fmin s) x)
+  = seq_fold_left_append fmin pos_inf s (Seq.create 1 x);
+    seq_fold_left_one fmin (seq_fmin s) x
